code/sha2-vec/Hacl.Impl.SHA2.Core.fsti
@@ -7,6 +7,7 @@ open Lib.IntTypes
 open Lib.Sequence
 open Lib.Buffer
 open Lib.IntVector
+open Lib.MultiBuffer
 open Spec.Hash.Definitions
 open Hacl.Hash.Definitions
 module Spec = Hacl.Spec.SHA2
@@ -18,20 +19,13 @@ val sha256: hash:lbuffer uint8 32ul -> len:size_t -> b:lbuffer uint8 len ->
                            as_seq h1 hash == Spec.hash #SHA2_256 (v len) (as_seq h0 b)))
 
 
-val sha256_4: r0:lbuffer uint8 32ul ->
-              r1:lbuffer uint8 32ul ->
-              r2:lbuffer uint8 32ul ->
-              r3:lbuffer uint8 32ul ->
-              len:size_t ->
-              b0:lbuffer uint8 len ->
-              b1:lbuffer uint8 len ->
-              b2:lbuffer uint8 len ->
-              b3:lbuffer uint8 len ->
+val sha256_4 (r0 r1 r2 r3: lbuffer uint8 32ul)
+             (len:size_t)
+             (b0 b1 b2 b3: lbuffer uint8 len) :
     Stack unit
-    (requires (fun h0 -> live h0 b0 /\ live h0 b1 /\ live h0 b2 /\ live h0 b3 /\ 
-                       live h0 r0 /\ live h0 r1 /\ live h0 r2 /\ live h0 r3 /\
-                       disjoint r0 r1 /\ disjoint r0 r2 /\ disjoint r0 r3 /\
-                       disjoint r1 r2 /\ disjoint r1 r3 /\ disjoint r2 r3))
+    (requires (fun h0 -> live4 h0 b0 b1 b2 b3 /\
+                       live4 h0 r0 r1 r2 r3 /\
+                       internally_disjoint4 r0 r1 r2 r3))
     (ensures (fun h0 _ h1 -> modifies (loc r0 |+| loc r1 |+| loc r2 |+| loc r3) h0 h1 /\
                            as_seq h1 r0 == Spec.hash #SHA2_256 (v len) (as_seq h0 b0) /\
                            as_seq h1 r1 == Spec.hash #SHA2_256 (v len) (as_seq h0 b1) /\
@@ -40,32 +34,19 @@ val sha256_4: r0:lbuffer uint8 32ul ->
 
 
 
-val sha256_8: r0:lbuffer uint8 32ul ->
-              r1:lbuffer uint8 32ul ->
-              r2:lbuffer uint8 32ul ->
-              r3:lbuffer uint8 32ul ->
-              r4:lbuffer uint8 32ul ->
-              r5:lbuffer uint8 32ul ->
-              r6:lbuffer uint8 32ul ->
-              r7:lbuffer uint8 32ul ->
-              len:size_t ->
-              b0:lbuffer uint8 len ->
-              b1:lbuffer uint8 len ->
-              b2:lbuffer uint8 len ->
-              b3:lbuffer uint8 len ->
-              b4:lbuffer uint8 len ->
-              b5:lbuffer uint8 len ->
-              b6:lbuffer uint8 len ->
-              b7:lbuffer uint8 len ->
+val sha256_8 (r0 r1 r2 r3 r4 r5 r6 r7 : lbuffer uint8 32ul)
+             (len:size_t)
+             (b0 b1 b2 b3 b4 b5 b6 b7 : lbuffer uint8 len) :
     Stack unit
-    (requires (fun h0 -> live h0 b0 /\ live h0 b1 /\ live h0 b2 /\ live h0 b3 /\ live h0 b4 /\ live h0 b5 /\ live h0 b6 /\ live h0 b7 /\  
-                       live h0 r0 /\ live h0 r1 /\ live h0 r2 /\ live h0 r3 /\ live h0 r4 /\ live h0 r5 /\ live h0 r6 /\ live h0 r7 /\
-                       disjoint r0 r1 /\ disjoint r0 r2 /\ disjoint r0 r3 /\
-                       disjoint r1 r2 /\ disjoint r1 r3 /\ disjoint r2 r3))
-    (ensures (fun h0 _ h1 -> modifies (loc r0 |+| loc r1 |+| loc r2 |+| loc r3) h0 h1 /\
+    (requires (fun h0 -> live8 h0 b0 b1 b2 b3 b4 b5 b6 b7 /\ live8 h0 r0 r1 r2 r3 r4 r5 r6 r7 /\
+                       internally_disjoint8 r0 r1 r2 r3 r4 r5 r6 r7))
+    (ensures (fun h0 _ h1 -> modifies (loc r0 |+| loc r1 |+| loc r2 |+| loc r3 |+| loc r4 |+| loc r5 |+| loc r6 |+| loc r7) h0 h1 /\
                            as_seq h1 r0 == Spec.hash #SHA2_256 (v len) (as_seq h0 b0) /\
                            as_seq h1 r1 == Spec.hash #SHA2_256 (v len) (as_seq h0 b1) /\
                            as_seq h1 r2 == Spec.hash #SHA2_256 (v len) (as_seq h0 b2) /\
-                           as_seq h1 r3 == Spec.hash #SHA2_256 (v len) (as_seq h0 b3)))
-
+                           as_seq h1 r3 == Spec.hash #SHA2_256 (v len) (as_seq h0 b3) /\
+                           as_seq h1 r4 == Spec.hash #SHA2_256 (v len) (as_seq h0 b4) /\
+                           as_seq h1 r5 == Spec.hash #SHA2_256 (v len) (as_seq h0 b5) /\
+                           as_seq h1 r6 == Spec.hash #SHA2_256 (v len) (as_seq h0 b6) /\
+                           as_seq h1 r7 == Spec.hash #SHA2_256 (v len) (as_seq h0 b7)))
 
